chore: namespace Zipper

SSA/Core/Framework/Zipper.lean
@@ -22,7 +22,7 @@ structure Zipper (Γ_in : Ctxt d.Ty) (eff : EffectKind) (Γ_mid : Ctxt d.Ty) (ty
   bot : Com d Γ_mid eff ty
 
 
--- namespace Zipper
+namespace Zipper
 variable {d}
 
 /-!
@@ -33,15 +33,15 @@ variable [TyDenote d.Ty] [DialectDenote d] [Monad d.m]
 
 /-- The denotation of a zipper is a composition of the denotations of the constituent
 `Lets` and `Com` -/
-def Zipper.denote (zip : Zipper d Γ_in eff Γ_out ty) (V_in : Valuation Γ_in) :
+def denote (zip : Zipper d Γ_in eff Γ_out ty) (V_in : Valuation Γ_in) :
     eff.toMonad d.m ⟦ty⟧ :=
   (zip.top.denote V_in) >>= zip.bot.denote
 
-@[simp] lemma Zipper.denote_mk {lets : Lets d Γ_in eff Γ_out} {com : Com d Γ_out eff ty} :
+@[simp] lemma denote_mk {lets : Lets d Γ_in eff Γ_out} {com : Com d Γ_out eff ty} :
     denote ⟨lets, com⟩ = fun V => (lets.denote V) >>= com.denote := rfl
 
 /-- Casting the intermediate context is not relevant for the denotation -/
-@[simp] lemma Zipper.denoteLets_eqRec_Γ_mid {zip : Zipper d Γ_in eff Γ_mid ty}
+@[simp] lemma denoteLets_eqRec_Γ_mid {zip : Zipper d Γ_in eff Γ_mid ty}
     (h : Γ_mid = Γ_mid') :
     denote (h ▸ zip) = zip.denote := by
   subst h; rfl
@@ -56,22 +56,22 @@ end Denote
 section ToCom
 
 /-- Recombine a zipper into a single program by adding the `lets` to the beginning of the `com` -/
-def Zipper.toCom (zip : Zipper d Γ_in eff Γ_mid ty) : Com d Γ_in eff ty :=
+def toCom (zip : Zipper d Γ_in eff Γ_mid ty) : Com d Γ_in eff ty :=
   go zip.top zip.bot
   where
     go : {Γ_mid : _} → Lets d Γ_in eff Γ_mid → Com d Γ_mid eff ty → Com d Γ_in eff ty
       | _, .nil, com          => com
       | _, .var body e, com  => go body (.var e com)
 
-@[simp] lemma Zipper.toCom_nil {com : Com d Γ eff ty} : Zipper.toCom ⟨.nil, com⟩ = com := rfl
-@[simp] lemma Zipper.toCom_var {lets : Lets d Γ_in eff Γ_mid} :
-    Zipper.toCom ⟨Lets.var lets e, com⟩ = Zipper.toCom ⟨lets, Com.var e com⟩ := rfl
+@[simp] lemma toCom_nil {com : Com d Γ eff ty} : toCom ⟨.nil, com⟩ = com := rfl
+@[simp] lemma toCom_var {lets : Lets d Γ_in eff Γ_mid} :
+    toCom ⟨Lets.var lets e, com⟩ = toCom ⟨lets, Com.var e com⟩ := rfl
 
 variable [TyDenote d.Ty] [DialectDenote d] [Monad d.m]
-@[simp] theorem Zipper.denote_toCom [LawfulMonad d.m] (zip : Zipper d Γ_in eff Γ_mid ty) :
+@[simp] theorem denote_toCom [LawfulMonad d.m] (zip : Zipper d Γ_in eff Γ_mid ty) :
     zip.toCom.denote = zip.denote := by
   rcases zip with ⟨lets, com⟩
-  funext Γv; induction lets <;> simp [Lets.denote, Zipper.denote, *]
+  funext Γv; induction lets <;> simp [Lets.denote, denote, *]
 
 end ToCom
 
@@ -81,7 +81,7 @@ variable [DecidableEq d.Ty]
 
 /-- Add a `Com` directly before the current position of a zipper, while reassigning every
 occurence of a given free variable (`v`) of `zip.com` to the output of the new `Com`  -/
-def Zipper.insertCom (zip : Zipper d Γ_in eff Γ_mid ty) (v : Var Γ_mid newTy)
+def insertCom (zip : Zipper d Γ_in eff Γ_mid ty) (v : Var Γ_mid newTy)
     (newCom : Com d Γ_mid eff newTy) : Zipper d Γ_in eff newCom.outContext ty :=
   let newTop := zip.top.addComToEnd newCom
   --  ^^^^^^ The combination of the previous `top` with the `newCom` inserted
@@ -96,7 +96,7 @@ zipper, while r eassigning every occurence of a given free variable (`v`) of
 
 This is a wrapper around `insertCom` (which expects `newCom` to have the same effect as `zip`)
 and `castPureToEff` -/
-def Zipper.insertPureCom (zip : Zipper d Γ_in eff Γ_mid ty) (v : Var Γ_mid newTy)
+def insertPureCom (zip : Zipper d Γ_in eff Γ_mid ty) (v : Var Γ_mid newTy)
     (newCom : Com d Γ_mid .pure newTy) : Zipper d Γ_in eff newCom.outContext ty :=
   (by simp : (newCom.castPureToEff eff).outContext = newCom.outContext)
     ▸ zip.insertCom v (newCom.castPureToEff eff)
@@ -105,7 +105,7 @@ def Zipper.insertPureCom (zip : Zipper d Γ_in eff Γ_mid ty) (v : Var Γ_mid ne
 section Lemmas
 variable [TyDenote d.Ty] [DialectDenote d] [Monad d.m]
 
-theorem Zipper.denote_insertCom {zip : Zipper d Γ_in eff Γ_mid ty₁}
+theorem denote_insertCom {zip : Zipper d Γ_in eff Γ_mid ty₁}
     {newCom : Com d _ eff newTy} [LawfulMonad d.m] :
     (zip.insertCom v newCom).denote = (fun (V_in : Valuation Γ_in) => do
       let V_mid ← zip.top.denote V_in
@@ -116,7 +116,7 @@ theorem Zipper.denote_insertCom {zip : Zipper d Γ_in eff Γ_mid ty₁}
   funext V
   simp [insertCom, Com.denoteLets_eq]
 
-theorem Zipper.denote_insertPureCom {zip : Zipper d Γ_in eff Γ_mid ty₁}
+theorem denote_insertPureCom {zip : Zipper d Γ_in eff Γ_mid ty₁}
     {newCom : Com d _ .pure newTy} [LawfulMonad d.m] :
     (zip.insertPureCom v newCom).denote = (fun (V_in : Valuation Γ_in) => do
       let V_mid ← zip.top.denote V_in
@@ -133,3 +133,4 @@ theorem Zipper.denote_insertPureCom {zip : Zipper d Γ_in eff Γ_mid ty₁}
   funext V; simp [insertPureCom, denote_insertCom, Valuation.comap, this]
 
 end Lemmas
+end InsertCom
